The following binomial identities are derived
\begin{gather*}
    m^n = \sum_{k=0}^{n} \sum_{j=0}^{k} \binom{n}{k} \binom{k}{j} (-1)^{k-j} m^j,\\
    m^n = \sum_{k=0}^{n} \sum_{j=0}^{k} \binom{n}{j} \binom{n-j}{k-j} (-1)^{k-j} m^j.\\
\end{gather*}
Moreover, above results are verified by means of specified Mathematica scripts available at
\href{https://github.com/kolosovpetro/PolynomialIdentitiesInvolvingPascalsTriangleRows/blob/develop/mathematica/PolynomialIdentitiesInvolvingPascalsTriangleRows.m}
{\texttt{github.com/kolosovpetro/PolynomialIdentitiesInvolvingPascalsTriangleRows}}.
